.

Computability/Constructions/Eval_Aux.lean
@@ -11,48 +11,41 @@ open Denumerable
 open Encodable
 open List
 
-
 section rfindOpt
 namespace Computability.Code
 
 theorem rfind'_eqv_rfind : ((Nat.unpaired fun a m => (Nat.rfind fun n => (fun m => m = 0) <$> eval O c (Nat.pair a (n + m))).map (· + m)) (Nat.pair x 0)) = (Nat.rfind fun n => (fun m => m = 0) <$> eval O c ⟪x, n⟫) := by
--- theorem rfind'_eqv_rfind : ((Nat.unpaired fun a m => (Nat.rfind fun n => (fun m => m = 0) <$> eval O c (Nat.pair a (n + m))).map (· + m)) ∘ (Nat.pair <$> (fun (n:ℕ)=>n) <*> Part.some 0)) x = (Nat.rfind fun n => (fun m => m = 0) <$> eval O c ⟪x, n⟫) := by
-  simp only [Nat.unpaired]
-  simp only [Nat.unpair_pair, add_zero, Part.map_eq_map]
+  simp only [Nat.unpaired, Nat.unpair_pair, add_zero, Part.map_eq_map]
   exact rfl
 
+section rfind
 /--`[code_rfind c](x)=smallest n s.t. [c](x,n)=0.`-/
--- def c_rfind : ℕ→ℕ := fun c => comp (rfind' c) (pair Computability.Code.id zero)
-def c_rfind : Computability.Code→Computability.Code := fun c => (rfind' c).comp (pair c_id zero)
-
+def c_rfind : Computability.Code→Computability.Code := λ c ↦ (rfind' c).comp (pair c_id zero)
 /-- Given a code `c` -/
-abbrev rfind (O:ℕ→ℕ) : Code→ℕ→.ℕ := fun c => fun a=> Nat.rfind fun n => (fun m => m = 0) <$> eval O c (Nat.pair a n)
-theorem c_rfind_prop : eval O (c_rfind c) a = (rfind O c a) := by
+abbrev rfind (O:ℕ→ℕ) : Code → ℕ →. ℕ := λ c ↦ λ a ↦ Nat.rfind λ n ↦ (λ m ↦ m = 0) <$> eval O c (Nat.pair a n)
+theorem c_rfind_ev : eval O (c_rfind c) a = rfind O c a := by
   unfold c_rfind
   unfold rfind
   rw [←rfind'_eqv_rfind]
   simp [eval,Seq.seq]
-
-theorem c_rfind_prop2 : eval O (c_rfind c) a = (Nat.rfind (fun x => n2b' <$> eval O c (Nat.pair a x))) := by
-  simp [c_rfind_prop]
+theorem c_rfind_ev' : eval O (c_rfind c) a = (Nat.rfind (fun x => n2b' <$> eval O c (Nat.pair a x))) := by
+  simp [c_rfind_ev]
   simp [rfind]
   unfold n2b'
   simp
+end rfind
 
 def c_ppred := c_rfind (c_if_eq'.comp₂ left (succ.comp right))
 @[simp] theorem c_ppred_ev : eval O c_ppred y = Nat.ppred y := by
   unfold c_ppred
-  simp [c_rfind_prop2]
+  simp [c_rfind_ev']
   simp [eval]
   simp [Seq.seq]
   cases y with
   | zero =>
     simp
     have : ¬ ((Nat.rfind fun x ↦ Part.some (n2b' 1))).Dom := by
-      simp
       simp [n2b']
-
-
     exact Part.eq_none_iff'.mpr this
   | succ n =>
     simp
@@ -74,7 +67,7 @@ theorem c_ofOption_ev (hc1:code_total O c) : eval O (c_ofOption c) x = ↑(n2o (
 def c_rfindOpt (c:Code) := (c_ofOption c).comp₂ c_id (c_rfind (c_isSome.comp (c)))
 @[simp] theorem c_rfindOpt_ev (hc1:code_total O c) : eval O (c_rfindOpt c) x =  Nat.rfindOpt (fun y => n2o $ (eval O c (Nat.pair x y)).get (hc1 (Nat.pair x y))) := by
   unfold c_rfindOpt
-  simp [c_rfind_prop2]
+  simp [c_rfind_ev']
   unfold rfindOpt
   simp [eval]
   simp [n2b']
